feat (data/finset) disjoint finsets

data/finset.lean
@@ -312,9 +312,6 @@ by simp [subset_iff] {contextual:=tt}; finish
 
 @[simp] theorem empty_inter (s : finset α) : ∅ ∩ s = ∅ := ext.2 $ by simp
 
-theorem inter_eq_empty_iff_disjoint {s₁ s₂ : finset α} : s₁ ∩ s₂ = ∅ ↔ s₁.1.disjoint s₂.1 :=
-by rw ← val_eq_zero; simp [inter_eq_zero_iff_disjoint]
-
 @[simp] theorem insert_inter_of_mem {s₁ s₂ : finset α} {a : α} (h : a ∈ s₂) :
   insert a s₁ ∩ s₂ = insert a (s₁ ∩ s₂) :=
 ext.2 $ by simp; intro x; constructor; finish
@@ -992,6 +989,64 @@ sort_eq _ _
 
 @[simp] theorem sort_to_finset [decidable_eq α] (s : finset α) : (sort r s).to_finset = s :=
 list.to_finset_eq (sort_nodup r s) ▸ eq_of_veq (sort_eq r s)
+
 end sort
+
+def disjoint (s t : finset α) : Prop := ∀ ⦃a⦄, a ∈ s → a ∈ t → false
+
+theorem disjoint.symm {s t : finset α} (d : disjoint s t) : disjoint t s
+| a i₂ i₁ := d i₁ i₂
+
+@[simp] theorem disjoint_comm {s t : finset α} : disjoint s t ↔ disjoint t s :=
+⟨disjoint.symm, disjoint.symm⟩
+
+theorem disjoint_left {s t : finset α} : disjoint s t ↔ ∀ {a}, a ∈ s → a ∉ t := iff.rfl
+
+theorem disjoint_right {s t : finset α} : disjoint s t ↔ ∀ {a}, a ∈ t → a ∉ s :=
+disjoint_comm
+
+theorem disjoint_iff_ne {s t : finset α} : disjoint s t ↔ ∀ a ∈ s, ∀ b ∈ t, a ≠ b :=
+by simp [disjoint_left, imp_not_comm]
+
+theorem disjoint_of_subset_left {s t u : finset α} (h : s ⊆ u) (d : disjoint u t) : disjoint s t
+| x m₁ := d (h m₁)
+
+theorem disjoint_of_subset_right {s t u : finset α} (h : t ⊆ u) (d : disjoint s u) : disjoint s t
+| x m m₁ := d m (h m₁)
+
+@[simp] theorem empty_disjoint (l : finset α) : disjoint ∅ l
+| a := (not_mem_empty a).elim
+
+@[simp] theorem singleton_disjoint {l : finset α} {a : α} : disjoint (singleton a) l ↔ a ∉ l :=
+by simp [disjoint]; refl
+
+@[simp] theorem disjoint_singleton {l : finset α} {a : α} : disjoint l (singleton a) ↔ a ∉ l :=
+by rw disjoint_comm; simp
+
+@[simp] theorem disjoint_insert_left [decidable_eq α] {a : α} {s t : finset α} :
+  disjoint (insert a s) t ↔ a ∉ t ∧ disjoint s t :=
+by simp [disjoint, or_imp_distrib, forall_and_distrib]; refl
+
+@[simp] theorem disjoint_insert_right [decidable_eq α] {a : α} {s t : finset α} :
+  disjoint s (insert a t) ↔ a ∉ s ∧ disjoint s t :=
+disjoint_comm.trans $ by simp [disjoint_insert_left]
+
+theorem inter_eq_empty_iff_disjoint [decidable_eq α] {s t : finset α} : s ∩ t = ∅ ↔ disjoint s t :=
+by simp [ext, mem_inter]; refl
+
+@[simp] theorem disjoint_union_left [decidable_eq α] {s t u : finset α} :
+  disjoint (s ∪ t) u ↔ disjoint s u ∧ disjoint t u :=
+by simp [disjoint, or_imp_distrib, forall_and_distrib]
+
+@[simp] theorem disjoint_union_right [decidable_eq α] {s t u : finset α} :
+  disjoint s (t ∪ u) ↔ disjoint s t ∧ disjoint s u :=
+by simp [disjoint, or_imp_distrib, forall_and_distrib]
+
+@[simp] theorem disjoint_val {s t : finset α} : multiset.disjoint s.1 t.1 ↔ disjoint s t :=
+by simp [disjoint, multiset.disjoint, mem_def]
+
+@[simp] theorem card_disjoint_union [decidable_eq α] {s t : finset α} :
+    disjoint s t → card (s ∪ t) = card s + card t :=
+finset.induction_on s (by simp) $ by simp {contextual := tt}
 
 end finset
